

Logarithms and Exponentials

Amos Thacker-Gwaltney

January 28, 2026

1 Definition of a Logarithm

if x and b are positive real numbers such that $b \neq 1$ then $y = \log_b x$ is called the logarithmic function base b , where:

$$(y = \log_b x) = (b^y = x)$$

* Given $y = \log_b x$, the value y is the exponent to which b must be raised to obtain x .

* The value of y is called the logarithm, b is called the base, and x is called the argument.

* The equations $y = \log_b x$ and $b^y = x$ both define the same relationship between x and y . The expression $y = \log_b x$ is called the logarithmic form and $x = b^y$ is called the exponential form.

2 The Use Case

Some exponential equations are impossible to solve by inspection.

in $5^x = 5$ the solution is $x = 1$
however, consider $5^x = 20$

We cannot find the value of x but we know it is between one and two. That said all exponential functions are one-to-one functions, so we can isolate x by performing the inverse operation of 5^x .

The inverse operation of an exponential function, base b , is the logarithmic function base b , which is defined above.

3 Converting Between Log. and Exp. Form

Questions:

$$\log_2 16 = 4 \quad (1)$$

$$\log_{10}\left(\frac{1}{100}\right) = -2 \quad (2)$$

$$\log_7 1 = 0 \quad (3)$$

Answers:

$$(2^4 = 16) = (\log_2 16 = 4) \quad (4)$$

$$(10^{-2} = \frac{1}{100}) = (\log_{10}\left(\frac{1}{100}\right) = -2) \quad (5)$$

$$(7^0 = 1) = (\log_7 1 = 0) \quad (6)$$

4 Common Logarithms

In many contexts the base of a logarithm will be excluded, this doesn't mean there is no base, it means that the base is ten. Base ten logarithms are called common logarithms. The notation for a log of base ten is the leftmost logarithm denoted below, the right log is for illustrating equivalency.

$$(y = \log x) = (y = \log_{10} x)$$

5 Natural Logarithm (ln)

The logarithmic function base e is called the natural logarithmic function. The natural logarithmic function is denoted below. You can think of the ln notation as log natural.

$$(y = \ln x) = (\log_e x = y)$$

6 Basic Properties of Logarithms

$$1 * \log_b 1 = 0 \text{ because } b^0 = 1$$

$$2 * \log_b b = 1 \text{ because } b^1 = b$$

$$3 * \log_b b^x = x \text{ because } b^x = b^x$$

4 * $b^{\log_b x} = x$ because $\log_b x = \log_b x$

Properties 3 and 4 follow from the fact that a logarithmic function is the inverse of an exponential function of the same base.

Given $f(x) = b^x$ and $f^{-1}(x) = \log_b x$

* $(f \circ f^{-1})(x) = b^{\log_b x} = x$ (Property 4)

* $(f^{-1} \circ f)(x) = \log_b(b^x) = x$ (Property 3)

7 Product Property of Logarithms

By definition, $y = \log_b x$ is equivalent to $b^y = x$. Because a logarithm is an exponent, the properties of exponents can be applied to logarithms. The first is called the product property of logarithms.

Let b , x , and y be positive real numbers where $b \neq 1$. Then

$$\log_b(xy) = \log_b x + \log_b y$$

The logarithm of a product equals the sum of the logarithms of the factors.

Proof:

* Let $M = \log_b x$, which implies $b^M = x$

* Let $N = \log_b y$, which implies $b^N = y$

* Then $xy = b^M b^N = b^{M+N}$

Writing the expression $xy = b^{M+N}$ in logarithmic form, we have,

$$\log_b(xy) = M + N$$

$$\log_b(xy) = \log_b x + \log_b y$$

Example:

$$\log_3(3 \cdot 9) = \log_3 3 + \log_3 9$$

$$\log_3 27 = 1 + 2$$

$$3 = 3$$

8 Quotient Property of Logarithms

\Longleftrightarrow means if and only if

This property is derived from the quotient rule of exponents which tells us that

$$\frac{b^M}{b^N} = b^{M-N} \Longleftrightarrow b \neq 0$$

. This property can be applied to logarithms due to the aforementioned relationship between a logarithm as an exponent value of its inverse exponential function. Let b, x, and y be positive real numbers where $b \neq 1$. Then

$$\log_b \frac{x}{y} = \log_b x - \log_b y$$

The logarithm of a quotient equals the difference of the numerator and the logarithm of the denominator.

Proof:

$$\begin{aligned} \log\left(\frac{1,000,000}{100}\right) &= \log 1,000,000 - \log 100 \\ \log 10,000 &= 6 - 2 \\ 4 &= 4 \end{aligned}$$

9 Power Property of Logarithms

The power property of exponents tells us that

$$(b^M)^N = b^{MN}$$

The same principle can be applied to logarithms.

Let b and x be positive real numbers where $b \neq 1$. Let p be any real number.

$$\log_b x^p = p \log_b x$$

Proof:

$$\begin{aligned} \log_2 4^2 &= 2 \log_2 4 \\ \log_2 16 &= 2 \cdot 2 \\ 4 &= 4 \end{aligned}$$

10 Graphing

Since a logarithmic function $y = \log_b x$ is the inverse of the corresponding function $y = b^x$, their graphs must be symmetric with respect to the line $y = x$.

The range of $y = b^x$ is the set of positive real numbers. As expected, the domain of its inverse function $y = \log_b x$ is the set of positive real numbers.

When you have a logarithm of the form

a. $f(x) = \log_2(2x + 4)$

b. $g(x) = \log_2(5 - x)$

c. $h(x) = \log(x^2 - 9)$

(a) solution:

$$f(x) = \log_2(2x + 4)$$

$$2x + 4 > 0$$

$$2x > -4$$

$$x > -2$$

The domain is $(-2, \infty)$

The vertical asymptote is $x = -2$

(b) solution:

$$g(x) = \log_2(5 - x)$$

$$5 - x > 0$$

$$-x > -5$$

$$x < 5$$

The domain is $(-\infty, 5)$

The vertical asymptote is $x = 5$

(c) solution:

$$h(x) = \log(x^2 - 9)$$

$$x^2 - 9 > 0$$

$$(x - 3)(x + 3) = 0$$

The domain is $(-\infty, -3) \cup (3, \infty)$

The vertical asymptotes are $x = -3$ and $x = 3$

11 Change of Base Formula

Let a and b be positive real numbers such that $a \neq 1$ and $b \neq 1$. Then for any positive real number x ,

$$\log_b x = \frac{\log_a x}{\log_a b}$$

The change-of-base formula converts a logarithm of one base to a ratio of logarithms of a different base. For the purpose of using a calculator, we often apply the change-of-base formula with base 10 or base e .

To derive the change-of-base formula, assume that a and b are positive real numbers with $a \neq 1$ and $b \neq 1$. Begin by letting $y = \log_b x$. If $y = \log_b x$, then

$$b^y = x$$

$$\log_a b^y = \log_a x$$

$$y \cdot \log_a b = \log_a x$$

$$y = \frac{\log_a x}{\log_a b}$$

$$\log_b x = \frac{\log_a x}{\log_a b}$$

12 Examples

$$3^{2y-2} = \frac{1}{3}^{y-7}$$

express the fractional base as a negative exponent.

$$3^{2y-2} = (3^{-1})^{y-7}$$

$$3^{2y-2} = 3^{-y+7}$$

$$2y - 2 = -y + 7$$

$$2y = -y + 9$$

$$3y = 9$$

$$y = 3$$

$$10^{4+8y} + 3,500 = 138,000$$

$$10^{4+8y} = 134,500$$

$$\log_{10} 10^{4+8y} = \log_{10} 134,500$$

to simplify the lvalue:

$$\log_{10} 10^{4+8y} = (10^y = 10^{4+8y}) = 4 + 8y$$

back to the problem:

$$4 + 8y = \log 134,500$$

$$8y = \log 134,500 - 4$$

$$y = \frac{\log 134,500 - 4}{8}$$

13 Equivalence Property of Exponential Expressions

if b , x , and y are real numbers with $b > 0$ and $n \neq 1$ then $b^x = b^y$ implies that $x = y$.

if two exponential equations with the same base are equal, then their exponents must be equal.

14 Solving Exponential Equations with Logarithms

- 1: Isolate the exponential expression on one side of the equation.
- 2: Take a logarithm of the same base on both sides of the equation.
- 3: Use the power property of logarithms to "bring down" the exponent.
- 4: Solve the resulting equation.